no admit inside any of the synchronisation steps.

concurrency/compiler/spawn_diagrams.v
@@ -211,7 +211,7 @@ Section SpawnDiagrams.
     Qed.
     Lemma permMapJoin_pair_inject_spawn:
       forall virtue1 virtue_new1 m1
-        m2 mu  th_perms1 th_perms2,
+             m2 mu  th_perms1 th_perms2,
         sub_map_pair virtue1 (snd (getMaxPerm m1)) ->
         sub_map_pair virtue_new1 (snd (getMaxPerm m1)) ->
         let ThreadPerm1 := computeMap_pair th_perms1 virtue1 in
@@ -236,14 +236,18 @@ Section SpawnDiagrams.
             permMapJoin_pair_inject_rel               
            the rpoof should be similar.*)
     Admitted.
-    Lemma concur_match_add_thread:
-      forall i f ocd st1 m1 st2 m2
+    (*The 3rd term has type "option (@compiler_index CC_correct0 Args0)" which should be coercible to
+ "option (@compiler_index CC_correct Args)".*)
+    Lemma concur_match_add_thread: 
+      forall {CC_correct : CompCert_correctness} {Args : ThreadSimulationArguments}
+        hb i f (ocd: option (@compiler_index CC_correct Args))
+        st1 m1 st2 m2
         (cnt1 : containsThread st1 i)
         (cnt2 : containsThread st2 i)
         c1 c2 th_perms11 th_perms12 th_perms21 th_perms22
         new_th_perms11 new_th_perms12 new_th_perms21 new_th_perms22
         b1 b2 ofs1 ofs2 arg1 arg2 delta,
-        concur_match ocd f st1 m1 st2 m2 ->
+        concur_match.concur_match hb ocd f st1 m1 st2 m2 ->
 
         
         let st1' := updThread cnt1 c1 (th_perms11, th_perms12) in
@@ -252,42 +256,42 @@ Section SpawnDiagrams.
         let st2'' := addThread st2' (Vptr b2 ofs2) arg2 (new_th_perms21,new_th_perms22) in
         
         forall (Hmem_compat1: mem_compatible(tpool:=OrdinalThreadPool) st1'' m1)
-          (Hmem_compat2: mem_compatible(tpool:=OrdinalThreadPool) st2'' m2)
-          
-          (Hlock_ppimage: perm_surj f (th_perms12) (th_perms22))
-          (Hlock_ppimage: perm_surj f (new_th_perms12) (new_th_perms22))
+               (Hmem_compat2: mem_compatible(tpool:=OrdinalThreadPool) st2'' m2)
+               
+               (Hlock_ppimage: perm_surj f (th_perms12) (th_perms22))
+               (Hlock_ppimage: perm_surj f (new_th_perms12) (new_th_perms22))
 
-          (* Two mem injects for the OLD thread *)
-          (Hlt1 : permMapLt (th_perms11) (getMaxPerm m1))
-          (Hlt2 : permMapLt (th_perms21) (getMaxPerm m2))
-          (Hinj_perms: Mem.inject f (restrPermMap Hlt1) (restrPermMap Hlt2))
-          
-          (Hlt1_lk : permMapLt (th_perms12) (getMaxPerm m1))
-          (Hlt2_lk : permMapLt (th_perms22) (getMaxPerm m2))
-          (Hinj_lock: Mem.inject f (restrPermMap Hlt1_lk) (restrPermMap Hlt2_lk))
+               (* Two mem injects for the OLD thread *)
+               (Hlt1 : permMapLt (th_perms11) (getMaxPerm m1))
+               (Hlt2 : permMapLt (th_perms21) (getMaxPerm m2))
+               (Hinj_perms: Mem.inject f (restrPermMap Hlt1) (restrPermMap Hlt2))
+               
+               (Hlt1_lk : permMapLt (th_perms12) (getMaxPerm m1))
+               (Hlt2_lk : permMapLt (th_perms22) (getMaxPerm m2))
+               (Hinj_lock: Mem.inject f (restrPermMap Hlt1_lk) (restrPermMap Hlt2_lk))
 
-          (* Two mem injects for the NEW thread *)
-          (Hlt1_new : permMapLt (new_th_perms11) (getMaxPerm m1))
-          (Hlt2_new : permMapLt (new_th_perms21) (getMaxPerm m2))
-          (Hinj_new_perms: Mem.inject f (restrPermMap Hlt1_new) (restrPermMap Hlt2_new))
-          
-          (Hlt1_lk_new : permMapLt (new_th_perms12) (getMaxPerm m1))
-          (Hlt2_lk_new : permMapLt (new_th_perms22) (getMaxPerm m2))
-          (Hinj_lock_new: Mem.inject f (restrPermMap Hlt1_lk_new) (restrPermMap Hlt2_lk_new))
-          
-          (Hinv1: invariant(tpool:=OrdinalThreadPool) st1'')
-          (Hinv2: invariant(tpool:=OrdinalThreadPool) st2'')
+               (* Two mem injects for the NEW thread *)
+               (Hlt1_new : permMapLt (new_th_perms11) (getMaxPerm m1))
+               (Hlt2_new : permMapLt (new_th_perms21) (getMaxPerm m2))
+               (Hinj_new_perms: Mem.inject f (restrPermMap Hlt1_new) (restrPermMap Hlt2_new))
+               
+               (Hlt1_lk_new : permMapLt (new_th_perms12) (getMaxPerm m1))
+               (Hlt2_lk_new : permMapLt (new_th_perms22) (getMaxPerm m2))
+               (Hinj_lock_new: Mem.inject f (restrPermMap Hlt1_lk_new) (restrPermMap Hlt2_lk_new))
+               
+               (Hinv1: invariant(tpool:=OrdinalThreadPool) st1'')
+               (Hinv2: invariant(tpool:=OrdinalThreadPool) st2'')
 
-          (* Match NEW thread *)
-          (Hthread_match: one_thread_match hb hb i ocd f  
-                                           c1 (restrPermMap Hlt1)
-                                           c2 (restrPermMap Hlt2))
+               (* Match NEW thread *)
+               (Hthread_match: one_thread_match hb hb i ocd f  
+                                                c1 (restrPermMap Hlt1)
+                                                c2 (restrPermMap Hlt2))
 
-          (* Match NEW thread *)
-          (Hinj_args: val_inject f arg1 arg2)
-          (Hinj_ptr: f b1 = Some (b2 , delta))
-          (Hinj_ptr: ofs2 = add ofs1 (repr delta)),
-          concur_match ocd f st1'' m1 st2'' m2.
+               (* Match NEW thread *)
+               (Hinj_args: val_inject f arg1 arg2)
+               (Hinj_ptr: f b1 = Some (b2 , delta))
+               (Hinj_ptr: ofs2 = add ofs1 (repr delta)),
+          concur_match.concur_match hb ocd f st1'' m1 st2'' m2.
     Proof.
       (*This should go in concur_match *)
     Admitted.
@@ -297,136 +301,176 @@ Section SpawnDiagrams.
     Admitted.
     (* probably go to advanced permissions *)
     
-      Definition mi_perm_perm_pair mu:= pair2_prop (mi_perm_perm mu).
-      Hint Unfold mi_perm_perm_pair:pair.
-      Definition dmap_map (dmp:delta_map): PMap.t _ :=
-        (fun _ : Z => None, dmp).
-      Definition dmap_map_pair := pair1 dmap_map.
-      Hint Unfold dmap_map_pair:pair.
-      Hint Unfold sub_map_pair: pair.
-      Lemma computeMap_mi_perm_perm_perfect_pair:
-        forall mu x1 y1 x2 y2,
+    Definition mi_perm_perm_pair mu:= pair2_prop (mi_perm_perm mu).
+    Hint Unfold mi_perm_perm_pair:pair.
+    Definition dmap_map (dmp:delta_map): PMap.t _ :=
+      (fun _ : Z => None, dmp).
+    Definition dmap_map_pair := pair1 dmap_map.
+    Hint Unfold dmap_map_pair:pair.
+    Hint Unfold sub_map_pair: pair.
+    Lemma computeMap_mi_perm_perm_perfect_pair:
+      forall mu x1 y1 x2 y2,
         maps_no_overlap_pair mu x1 (dmap_map_pair y1) ->
-       mi_perm_perm_pair mu x1 x2 ->
-       perm_perfect_image_dmap_pair mu y1 y2 ->
-       mi_perm_perm_pair mu (computeMap_pair x1 y1) (computeMap_pair x2 y2).
-      Proof.
-        intros mu. solve_pair.
-        apply computeMap_mi_perm_perm_perfect.
-      Qed.
-      Lemma maps_no_overlap_Lt_pair:
-          forall (mu : meminj) bound,
-            map_no_overlap mu bound ->
-            forall x y,
-            permMapLt_pair x bound ->
-            sub_map_pair y (snd bound) ->
-            maps_no_overlap_pair mu x (dmap_map_pair y).
-        Proof.
-          intros mu bound Hno_over.
-          solve_pair.
-          intros; eapply maps_no_overlap_Lt; eauto.
-        Qed.
-        Lemma empty_LT_pair:
-            forall pmap,
-              permMapLt_pair (pair0 empty_map) pmap.
-          Proof. intros; solve_pair. apply empty_LT. Qed.
-          Lemma mi_perm_perm_empty:
-          forall mu, mi_perm_perm mu (empty_map) (empty_map).
-        Proof. intros ? ? **.
-               rewrite empty_is_empty in H0; inv H0. Qed.
-        Lemma mi_perm_perm_empty_pair:
-          forall mu,
-          mi_perm_perm_pair mu (pair0 empty_map) (pair0 empty_map).
-        Proof. intros mu; solve_pair. apply mi_perm_perm_empty. Qed.
-        Hint Unfold injects_dmap_pair: pair.
-        Lemma inject_perm_perfect_image_dmap_pair:
-          forall (mu : meminj) (m1 m2 : mem), 
-            Mem.inject mu m1 m2 ->
-            forall (dmap : Pair delta_map),
-            option_implication_dmap_access_pair dmap (getMaxPerm m1) ->
-            injects_dmap_pair mu dmap ->
-            perm_perfect_image_dmap_pair mu dmap
-                                         (pair1 (tree_map_inject_over_mem m2 mu) dmap).
-        Proof.
-          intros ??? ?.
-          solve_pair. intros; eapply inject_perm_perfect_image_dmap; eauto.
-        Qed.
-        (* end of advanced_permissions's lemmas*)
-Lemma mi_inj_mi_perm_perm_Cur_backwards:
-            forall mu p1 p2 m1 m2 Hlt1 Hlt2,
-            Mem.mem_inj mu (@restrPermMap p1 m1 Hlt1)
-                        (@restrPermMap p2 m2 Hlt2) ->
-            mi_perm_perm mu p1 p2.
-          Proof.
-            intros. apply mi_inj_mi_perm_perm_Cur in H.
-            do 2 rewrite getCur_restr in H; auto.
-          Qed.
+        mi_perm_perm_pair mu x1 x2 ->
+        perm_perfect_image_dmap_pair mu y1 y2 ->
+        mi_perm_perm_pair mu (computeMap_pair x1 y1) (computeMap_pair x2 y2).
+    Proof.
+      intros mu. solve_pair.
+      apply computeMap_mi_perm_perm_perfect.
+    Qed.
+    Lemma maps_no_overlap_Lt_pair:
+      forall (mu : meminj) bound,
+        map_no_overlap mu bound ->
+        forall x y,
+          permMapLt_pair x bound ->
+          sub_map_pair y (snd bound) ->
+          maps_no_overlap_pair mu x (dmap_map_pair y).
+    Proof.
+      intros mu bound Hno_over.
+      solve_pair.
+      intros; eapply maps_no_overlap_Lt; eauto.
+    Qed.
+    Lemma empty_LT_pair:
+      forall pmap,
+        permMapLt_pair (pair0 empty_map) pmap.
+    Proof. intros; solve_pair. apply empty_LT. Qed.
+    Lemma mi_perm_perm_empty:
+      forall mu, mi_perm_perm mu (empty_map) (empty_map).
+    Proof. intros ? ? **.
+           rewrite empty_is_empty in H0; inv H0. Qed.
+    Lemma mi_perm_perm_empty_pair:
+      forall mu,
+        mi_perm_perm_pair mu (pair0 empty_map) (pair0 empty_map).
+    Proof. intros mu; solve_pair. apply mi_perm_perm_empty. Qed.
+    Hint Unfold injects_dmap_pair: pair.
+    Lemma inject_perm_perfect_image_dmap_pair:
+      forall (mu : meminj) (m1 m2 : mem), 
+        Mem.inject mu m1 m2 ->
+        forall (dmap : Pair delta_map),
+          option_implication_dmap_access_pair dmap (getMaxPerm m1) ->
+          injects_dmap_pair mu dmap ->
+          perm_perfect_image_dmap_pair mu dmap
+                                       (pair1 (tree_map_inject_over_mem m2 mu) dmap).
+    Proof.
+      intros ??? ?.
+      solve_pair. intros; eapply inject_perm_perfect_image_dmap; eauto.
+    Qed.
+    (* end of advanced_permissions's lemmas*)
+    Lemma mi_inj_mi_perm_perm_Cur_backwards:
+      forall mu p1 p2 m1 m2 Hlt1 Hlt2,
+        Mem.mem_inj mu (@restrPermMap p1 m1 Hlt1)
+                    (@restrPermMap p2 m2 Hlt2) ->
+        mi_perm_perm mu p1 p2.
+    Proof.
+      intros. apply mi_inj_mi_perm_perm_Cur in H.
+      do 2 rewrite getCur_restr in H; auto.
+    Qed.
     
-      Definition mi_memval_perm_pair mu x cont1 cont2:=
-        pair1_prop (fun x=> mi_memval_perm mu x cont1 cont2) x.
-      
-          Definition mi_perm_inv_perm_pair mu pp1 pp2 m:=
-            pair2_prop (fun p1 p2 => mi_perm_inv_perm mu p1 p2 m) pp1 pp2.
-          Lemma mi_memval_perm_computeMap_Lt_pair:
-            forall mu cont1 cont2 p p',
-            mi_memval_perm_pair mu p cont1 cont2 ->
-            permMapLt_pair2 p' p ->
-            mi_memval_perm_pair mu p' cont1 cont2.
-          Proof.
-            unfold mi_memval_perm_pair,permMapLt_pair2.
-            intros ? ? ?. solve_pair.
-            eapply mi_memval_perm_computeMap_Lt.
-          Qed.
-          Lemma mi_inj_mi_memval_perm_backwards:
-              forall (f : meminj) (m1 m2 : mem) p1 p2 Hlt1 Hlt2,
-                Mem.mem_inj f
-                            (@restrPermMap p1 m1 Hlt1)
-                            (@restrPermMap p2 m2 Hlt2) ->
-                mi_memval_perm f p1
-                               (Mem.mem_contents m1) (Mem.mem_contents m2).
-            Proof.
-              intros. eapply mi_inj_mi_memval_perm in H.
-              rewrite getCur_restr in H. simpl in H; eauto.
-            Qed.      
-            Lemma mi_perm_inv_perm_compute_pair:
-              forall mu m1 m2 perm1 perm2 v Hlt11 Hlt12 Hlt21 Hlt22,
-              Mem.inject mu (@restrPermMap (fst perm1) m1 Hlt11)
-                         (@restrPermMap (fst perm2) m2 Hlt21) ->
-              Mem.inject mu (@restrPermMap (snd perm1) m1 Hlt12)
-                         (@restrPermMap (snd perm2) m2 Hlt22) ->
-              sub_map_pair v (snd (getMaxPerm m1)) ->
-              mi_perm_inv_perm_pair
-                mu
-                (computeMap_pair perm1 v)
-                (computeMap_pair perm2
-                                 (pair1 (tree_map_inject_over_mem m2 mu) v)) m1.
-            Proof.
-              intros. split.
-              - simpl; erewrite tree_map_inject_restr.
-                eapply (mi_perm_inv_perm_compute);
-                  try (symmetry; apply getCur_restr);
-                  eauto.
-                + rewrite restr_Max_eq; apply H1.
-                + eapply restr_Max_equiv.
-              - simpl; erewrite tree_map_inject_restr.
-                eapply (mi_perm_inv_perm_compute);
-                  try (symmetry; apply getCur_restr);
-                  eauto.
-                + rewrite restr_Max_eq; apply H1.
-                + eapply restr_Max_equiv.
-            Qed.
-            Lemma inject_empty:
-            forall mu m1 m2 Hlt1 Hlt2,
-               Mem.inject mu m1 m2 ->
-              Mem.inject mu (@restrPermMap empty_map m1 Hlt1)
-                         (@restrPermMap empty_map m2 Hlt2).
-          Proof.
-            intros; eapply inject_restr; auto.
-            - apply mi_perm_perm_empty.
-            - intros ? **. rewrite  empty_is_empty in H1; inv H1.
-            -  intros ? **. rewrite  empty_is_empty in H1; inv H1.
-          Qed.
-            Lemma spawn_step_diagram_self Sem tid m1 m2:
+    Definition mi_memval_perm_pair mu x cont1 cont2:=
+      pair1_prop (fun x=> mi_memval_perm mu x cont1 cont2) x.
+    
+    Definition mi_perm_inv_perm_pair mu pp1 pp2 m:=
+      pair2_prop (fun p1 p2 => mi_perm_inv_perm mu p1 p2 m) pp1 pp2.
+    Lemma mi_memval_perm_computeMap_Lt_pair:
+      forall mu cont1 cont2 p p',
+        mi_memval_perm_pair mu p cont1 cont2 ->
+        permMapLt_pair2 p' p ->
+        mi_memval_perm_pair mu p' cont1 cont2.
+    Proof.
+      unfold mi_memval_perm_pair,permMapLt_pair2.
+      intros ? ? ?. solve_pair.
+      eapply mi_memval_perm_computeMap_Lt.
+    Qed.
+    Lemma mi_inj_mi_memval_perm_backwards:
+      forall (f : meminj) (m1 m2 : mem) p1 p2 Hlt1 Hlt2,
+        Mem.mem_inj f
+                    (@restrPermMap p1 m1 Hlt1)
+                    (@restrPermMap p2 m2 Hlt2) ->
+        mi_memval_perm f p1
+                       (Mem.mem_contents m1) (Mem.mem_contents m2).
+    Proof.
+      intros. eapply mi_inj_mi_memval_perm in H.
+      rewrite getCur_restr in H. simpl in H; eauto.
+    Qed.      
+    Lemma mi_perm_inv_perm_compute_pair:
+      forall mu m1 m2 perm1 perm2 v Hlt11 Hlt12 Hlt21 Hlt22,
+        Mem.inject mu (@restrPermMap (fst perm1) m1 Hlt11)
+                   (@restrPermMap (fst perm2) m2 Hlt21) ->
+        Mem.inject mu (@restrPermMap (snd perm1) m1 Hlt12)
+                   (@restrPermMap (snd perm2) m2 Hlt22) ->
+        sub_map_pair v (snd (getMaxPerm m1)) ->
+        mi_perm_inv_perm_pair
+          mu
+          (computeMap_pair perm1 v)
+          (computeMap_pair perm2
+                           (pair1 (tree_map_inject_over_mem m2 mu) v)) m1.
+    Proof.
+      intros. split.
+      - simpl; erewrite tree_map_inject_restr.
+        eapply (mi_perm_inv_perm_compute);
+          try (symmetry; apply getCur_restr);
+          eauto.
+        + rewrite restr_Max_eq; apply H1.
+        + eapply restr_Max_equiv.
+      - simpl; erewrite tree_map_inject_restr.
+        eapply (mi_perm_inv_perm_compute);
+          try (symmetry; apply getCur_restr);
+          eauto.
+        + rewrite restr_Max_eq; apply H1.
+        + eapply restr_Max_equiv.
+    Qed.
+    Lemma inject_empty:
+      forall mu m1 m2 Hlt1 Hlt2,
+        Mem.inject mu m1 m2 ->
+        Mem.inject mu (@restrPermMap empty_map m1 Hlt1)
+                   (@restrPermMap empty_map m2 Hlt2).
+    Proof.
+      intros; eapply inject_restr; auto.
+      - apply mi_perm_perm_empty.
+      - intros ? **. rewrite  empty_is_empty in H1; inv H1.
+      -  intros ? **. rewrite  empty_is_empty in H1; inv H1.
+    Qed.
+    
+    (*synchronisation_steps_semantics*)
+    
+    Inductive spawn: val -> mem -> delta_map -> mem -> Prop :=
+      SpawnAngel: forall b ofs dpm m m' new_perms,
+        new_perms = computeMap (getCurPerm m) dpm ->
+        spawn (Vptr b ofs) m dpm m'.
+    Inductive extcall_spawn : Events.extcall_sem:=
+      ExtCallSpawn : forall 
+        (ge : Senv.t) (m m' m'' m''' : mem)
+        (b : block) (ofs : ptrofs) arg
+        (e : list Events.mem_effect)
+        (dpm : delta_map)
+        (e' : list Events.mem_effect),
+        mem_interference m e m' ->
+        spawn (Vptr b ofs) m' dpm m'' ->
+        mem_interference m'' e' m''' ->
+        extcall_spawn ge (Vptr b ofs::arg :: nil)
+                      m (Events.Event_acq_rel e dpm e' :: nil)
+                      Vundef m'''.
+    Axiom SpawnExists
+      : forall (ge : Senv.t) (args : list val) (m : mem) (ev : Events.trace) 
+          (r : val) (m' : mem),
+        Events.external_functions_sem "spawn" CREATE_SIG ge args m ev r m' =
+        extcall_spawn ge args m ev r m'.
+    Lemma spawn_is_consec: consecutive_sem "spawn" CREATE_SIG.
+    Admitted. 
+    Lemma spawn_doesnt_return: doesnt_return CREATE.
+    Admitted.
+    Lemma invariant_add_thread:
+            forall Sem (st st': @ThreadPool.t dryResources Sem OrdinalThreadPool)
+              h c old_th_perm  new_th_perm f_ptr arg
+              (Hcnt:ThreadPool.containsThread st h),
+      st' = ThreadPool.addThread
+              (ThreadPool.updThread Hcnt c old_th_perm)
+              f_ptr arg new_th_perm ->
+      invariant st ->
+      permMapJoin_pair new_th_perm old_th_perm  (getThreadR Hcnt) ->
+      invariant st'.
+          Admitted.
+    Lemma spawn_step_diagram_self Sem tid m1 m2:
       let CoreSem:= sem_coresem Sem in
       forall (SelfSim: (self_simulation (@semC Sem) CoreSem))
         virtue1 virtue_new1  cd
@@ -462,14 +506,14 @@ Lemma mi_inj_mi_perm_perm_Cur_backwards:
         let st1':= (ThreadPool.updThread cnt1 (Kresume sum_state1 Vundef) ThreadPerm1) in
         let st1'':= (ThreadPool.addThread st1' (Vptr b1 ofs) arg newThreadPerm1) in
         forall (Hcmpt : mem_compatible  st1'' m1)
-          (Hinv' : invariant st1'')
-          (Hangel_bound: sub_map_pair virtue1 (snd (getMaxPerm m1)))
-          (Hangel_bound_new : sub_map_pair virtue_new1 (snd (getMaxPerm m1)))
-          (Amatch : match_self (code_inject _ _ SelfSim) mu th_state1 m1 th_state2 m2)
-          (Hmatch_mem: match_mem mu m1 m2)
-          (Hat_external: semantics.at_external CoreSem th_state1 m1 =
-                         Some (CREATE, (Vptr b1 ofs :: arg :: nil)%list))
-          (Hjoin_angel: permMapJoin_pair newThreadPerm1 ThreadPerm1 (getThreadR cnt1)),
+               (Hinv' : invariant st1'')
+               (Hangel_bound: sub_map_pair virtue1 (snd (getMaxPerm m1)))
+               (Hangel_bound_new : sub_map_pair virtue_new1 (snd (getMaxPerm m1)))
+               (Amatch : match_self (code_inject _ _ SelfSim) mu th_state1 m1 th_state2 m2)
+               (Hmatch_mem: match_mem mu m1 m2)
+               (Hat_external: semantics.at_external CoreSem th_state1 m1 =
+                              Some (CREATE, (Vptr b1 ofs :: arg :: nil)%list))
+               (Hjoin_angel: permMapJoin_pair newThreadPerm1 ThreadPerm1 (getThreadR cnt1)),
 
         exists evnt2 (st2'' : t) m2',
           let evnt:= build_spwan_event (b1, unsigned ofs)
@@ -571,12 +615,12 @@ Lemma mi_inj_mi_perm_perm_Cur_backwards:
           + eapply no_overlap_mem_perm, Hinj.
           + exact (empty_LT_pair _).
           + eapply Hangel_bound_new.
-      - exact (mi_perm_perm_empty_pair _).
-      - eapply inject_perm_perfect_image_dmap_pair; eauto.
-        + eapply sub_map_implication_dmap_pair; eauto.
-        + eapply full_inject_dmap_pair; eauto.
-          eapply CMatch.
-          eapply join_dmap_valid_pair, Hangel_bound_new. }
+        - exact (mi_perm_perm_empty_pair _).
+        - eapply inject_perm_perfect_image_dmap_pair; eauto.
+          + eapply sub_map_implication_dmap_pair; eauto.
+          + eapply full_inject_dmap_pair; eauto.
+            eapply CMatch.
+            eapply join_dmap_valid_pair, Hangel_bound_new. }
       
       assert (Hmi_perm_perm: mi_perm_perm_pair mu ThreadPerm1 ThreadPerm2).
       { eapply computeMap_mi_perm_perm_perfect_pair.
@@ -588,41 +632,41 @@ Lemma mi_inj_mi_perm_perm_Cur_backwards:
             eauto.
           + apply Hinj_th.
           + apply Hinj_lock.
-      - eapply inject_perm_perfect_image_dmap_pair; eauto.
-        + eapply sub_map_implication_dmap_pair; eauto.
-        + eapply full_inject_dmap_pair; eauto.
-          eapply CMatch.
-          eapply join_dmap_valid_pair, Hangel_bound. }
+        - eapply inject_perm_perfect_image_dmap_pair; eauto.
+          + eapply sub_map_implication_dmap_pair; eauto.
+          + eapply full_inject_dmap_pair; eauto.
+            eapply CMatch.
+            eapply join_dmap_valid_pair, Hangel_bound. }
 
-            
-          assert (Hmemval:
-                    mi_memval_perm_pair mu ThreadPerm1
-                                        (Mem.mem_contents m1) (Mem.mem_contents m2)).
-          { eapply mi_memval_perm_computeMap_Lt_pair.
-            - split; eapply mi_inj_mi_memval_perm_backwards.
-              + eapply Hinj_th.
-              + eapply Hinj_lock.  
-            - eapply permMapJoin_lt_pair2; eauto. }
-          
-          assert (Hmemval_new:
-                    mi_memval_perm_pair mu newThreadPerm1
-                                        (Mem.mem_contents m1) (Mem.mem_contents m2)).
-          { eapply mi_memval_perm_computeMap_Lt_pair.
-            - split; eapply mi_inj_mi_memval_perm_backwards.
-              + eapply Hinj_th.
-              + eapply Hinj_lock.  
-            - eapply permMapJoin_lt_pair2, permMapJoin_pair_comm; eauto. }
+      
+      assert (Hmemval:
+                mi_memval_perm_pair mu ThreadPerm1
+                                    (Mem.mem_contents m1) (Mem.mem_contents m2)).
+      { eapply mi_memval_perm_computeMap_Lt_pair.
+        - split; eapply mi_inj_mi_memval_perm_backwards.
+          + eapply Hinj_th.
+          + eapply Hinj_lock.  
+        - eapply permMapJoin_lt_pair2; eauto. }
+      
+      assert (Hmemval_new:
+                mi_memval_perm_pair mu newThreadPerm1
+                                    (Mem.mem_contents m1) (Mem.mem_contents m2)).
+      { eapply mi_memval_perm_computeMap_Lt_pair.
+        - split; eapply mi_inj_mi_memval_perm_backwards.
+          + eapply Hinj_th.
+          + eapply Hinj_lock.  
+        - eapply permMapJoin_lt_pair2, permMapJoin_pair_comm; eauto. }
 
-          assert (Hmi_perm_inv_perm: (mi_perm_inv_perm_pair
-                                        mu ThreadPerm1
-                                        ThreadPerm2 m1)) by
-              (eapply mi_perm_inv_perm_compute_pair; eauto).
-          
-          assert (Hmi_perm_inv_perm_new: (mi_perm_inv_perm_pair
+      assert (Hmi_perm_inv_perm: (mi_perm_inv_perm_pair
+                                    mu ThreadPerm1
+                                    ThreadPerm2 m1)) by
+          (eapply mi_perm_inv_perm_compute_pair; eauto).
+      
+      assert (Hmi_perm_inv_perm_new: (mi_perm_inv_perm_pair
                                         mu newThreadPerm1
                                         newThreadPerm2 m1)).
-          { eapply mi_perm_inv_perm_compute_pair; eauto;
-              eapply inject_empty; eauto. }
+      { eapply mi_perm_inv_perm_compute_pair; eauto;
+          eapply inject_empty; eauto. }
 
       assert (Hinj': Mem.inject mu (restrPermMap Hlt1') (restrPermMap Hlt2')).
       { apply inject_restr; simpl; eauto.
@@ -652,16 +696,16 @@ Lemma mi_inj_mi_perm_perm_Cur_backwards:
       exists event2, st2'', m2.  
       repeat weak_split. (* 4 goal*)
       - !goal(concur_match _ _ _ _ _ _ ).
-
-        unshelve eapply concur_match_add_thread
+        
+        unshelve eapply (concur_match_add_thread hb tid mu cd st1)
           with (Hlt1:=Hlt1')
-            (Hlt2:=Hlt2')
-            (Hlt1_lk:=Hlt1_lk')
-            (Hlt2_lk:=Hlt2_lk')
-            (Hlt1_new:=Hlt1_new)
-            (Hlt2_new:=Hlt2_new)
-            (Hlt1_lk_new:=Hlt1_lk_new)
-            (Hlt2_lk_new:=Hlt2_lk_new); eauto;
+               (Hlt2:=Hlt2')
+               (Hlt1_lk:=Hlt1_lk')
+               (Hlt2_lk:=Hlt2_lk')
+               (Hlt1_new:=Hlt1_new)
+               (Hlt2_new:=Hlt2_new)
+               (Hlt1_lk_new:=Hlt1_lk_new)
+               (Hlt2_lk_new:=Hlt2_lk_new); eauto;
           subst ThreadPerm1 ThreadPerm2; simpl.
         + !goal(perm_surj _ _ _).
           eapply perm_surj_compute.
@@ -680,7 +724,10 @@ Lemma mi_inj_mi_perm_perm_Cur_backwards:
             -- eapply full_inject_dmap.
                ++ eapply CMatch.
                ++ eapply join_dmap_valid; eapply Hangel_bound_new.
-        + !goal(invariant _). admit. (* HERE sat *)
+        + !goal(invariant _).
+          eapply invariant_add_thread; eauto.
+          reflexivity.
+          apply CMatch.
         + !context_goal one_thread_match. shelve.
           
       - subst event2. repeat econstructor; eauto.
@@ -694,7 +741,7 @@ Lemma mi_inj_mi_perm_perm_Cur_backwards:
           |- syncStep _ _ _ _ _ ?ev =>
           match type of ev with
             ?T => evar (ev_new: T);
-                   replace ev with ev_new; unfold ev_new
+                    replace ev with ev_new; unfold ev_new
           end
         end.
 
@@ -704,11 +751,11 @@ Lemma mi_inj_mi_perm_perm_Cur_backwards:
           | |- _ => eauto; try reflexivity
           end.
         + eapply inject_virtue_sub_map_pair'; eauto. (*
-          * apply Hinj_lock.
-          * apply Hangel_bound. *)
+                                                      * apply Hinj_lock.
+                                                      * apply Hangel_bound. *)
         + eapply inject_virtue_sub_map_pair'; eauto. (*
-          * apply Hinj_lock.
-          * apply Hangel_bound_new. *)
+                                                      * apply Hinj_lock.
+                                                      * apply Hangel_bound_new. *)
         + eapply CMatch.
         + !goal (semantics.at_external _ _ _ = Some (CREATE, _)).
           { eapply at_external_sum_sem; eauto. }
@@ -731,7 +778,7 @@ Lemma mi_inj_mi_perm_perm_Cur_backwards:
               
               unshelve (eapply CMatch in Htid_neq' as Hthmatch); simpl;
                 eauto.
-            (*  + rewrite getMax_restr; eauto.
+              (*  + rewrite getMax_restr; eauto.
               + rewrite getMax_restr; eauto.*)
               + rewrite Hget_th_state1, Hget_th_state2 in Hthmatch.
                 unshelve (repeat erewrite <- restrPermMap_idempotent_eq in Hthmatch);
@@ -799,11 +846,9 @@ Lemma mi_inj_mi_perm_perm_Cur_backwards:
 
                      Unshelve.
                      all: simpl;eauto. }
-        
-
           
-    Admitted.
-
+    Qed.
+    
     Lemma spawn_step_diagram_compiled:
       let hybrid_sem:= (sem_coresem (HybridSem (Some hb))) in
       forall m1 m2 m10 virtue1 virtue_new1  cd
@@ -811,7 +856,7 @@ Lemma mi_inj_mi_perm_perm_Cur_backwards:
         (st2 : ThreadPool (Some (S hb)))
         (cnt1 : ThreadPool.containsThread(Sem:=HybridSem _) st1 hb)
         (cnt2 : containsThread(Sem:=HybridSem _) st2 hb)
-        (c : semC) (b1 : block) (ofs : int) arg
+        (b1 : block) (ofs : int) arg
         Hcnt1 Hcnt2 code1 code2
         (Hsame_cnt: same_cnt hb st1 st2 Hcnt1 Hcnt2)
         (CMatch: concur_match (Some cd) mu st1 m1 st2 m2)
@@ -830,16 +875,16 @@ Lemma mi_inj_mi_perm_perm_Cur_backwards:
         let ThreadPerm1:= (computeMap_pair (getThreadR cnt1) virtue1) in
         let newThreadPerm1:= (computeMap_pair (pair0 empty_map) virtue_new1) in
 
-        let st1':= (ThreadPool.updThread cnt1 (Kresume c Vundef) ThreadPerm1) in
+        let st1':= (ThreadPool.updThread cnt1 (Kresume (SST code1) Vundef) ThreadPerm1) in
         let st1'':= (ThreadPool.addThread st1' (Vptr b1 ofs) arg newThreadPerm1) in
         forall (Hcmpt : mem_compatible  st1'' m1)
-               (Hinv' : invariant st1'')
-               (Hangel_bound: pair21_prop sub_map virtue1 (snd (getMaxPerm m1)))
-               (Hangel_bound_new : pair21_prop sub_map virtue_new1 (snd (getMaxPerm m1)))
-               (Hat_external: semantics.at_external hybrid_sem (SST code1) m1 =
-                              Some (CREATE, (Vptr b1 ofs :: arg :: nil)%list))
-               (Hjoin_angel: permMapJoin_pair newThreadPerm1 ThreadPerm1 (getThreadR cnt1))
-               (Hstrict: strict_evolution_diagram cd mu code1 m10 m1 code2 m2),
+          (Hinv' : invariant st1'')
+          (Hangel_bound: pair21_prop sub_map virtue1 (snd (getMaxPerm m1)))
+          (Hangel_bound_new : pair21_prop sub_map virtue_new1 (snd (getMaxPerm m1)))
+          (Hat_external: semantics.at_external hybrid_sem (SST code1) m1 =
+                         Some (CREATE, (Vptr b1 ofs :: arg :: nil)%list))
+          (Hjoin_angel: permMapJoin_pair newThreadPerm1 ThreadPerm1 (getThreadR cnt1))
+          (Hstrict: strict_evolution_diagram cd mu code1 m10 m1 code2 m2),
 
         exists evnt2 (st2'' : t) m2',
           let evnt:= build_spwan_event (b1, unsigned ofs)
@@ -922,6 +967,107 @@ Lemma mi_inj_mi_perm_perm_Cur_backwards:
       forward_state_cmpt_all.
       rename Hcmpt_update into Hcmpt2'.
       rename Hcmpt_update0 into Hcmpt1'.
+
+      assert (Hlt1': permMapLt_pair (ThreadPerm1) (getMaxPerm m1)) by
+          solve_permMapLt_pair.
+      destruct Hlt1' as [Hlt1' Hlt1_lk']. 
+      assert (Hlt2': permMapLt_pair (ThreadPerm2) (getMaxPerm m2)) by
+          solve_permMapLt_pair.
+      destruct Hlt2' as [Hlt2' Hlt2_lk'].
+      assert (Hlt1_new: permMapLt_pair (newThreadPerm1) (getMaxPerm m1)) by
+          solve_permMapLt_pair.
+      destruct Hlt1_new as [Hlt1_new Hlt1_lk_new]. 
+      assert (Hlt2_new: permMapLt_pair (newThreadPerm2) (getMaxPerm m2)) by
+          solve_permMapLt_pair.
+      destruct Hlt2_new as [Hlt2_new Hlt2_lk_new].
+      simpl in *.
+
+      assert (Hmi_perm_perm_new: mi_perm_perm_pair mu newThreadPerm1 newThreadPerm2).
+      { eapply computeMap_mi_perm_perm_perfect_pair.
+        - eapply maps_no_overlap_Lt_pair; eauto.
+          + eapply no_overlap_mem_perm, Hinj'.
+          + exact (empty_LT_pair _).
+          + eapply Hangel_bound_new.
+        - exact (mi_perm_perm_empty_pair _).
+        - eapply inject_perm_perfect_image_dmap_pair; eauto.
+          + eapply sub_map_implication_dmap_pair; eauto.
+          + eapply full_inject_dmap_pair; eauto.
+            eapply CMatch.
+            eapply join_dmap_valid_pair, Hangel_bound_new. }
+      
+      assert (Hmi_perm_perm: mi_perm_perm_pair mu ThreadPerm1 ThreadPerm2).
+      { eapply computeMap_mi_perm_perm_perfect_pair.
+        - eapply maps_no_overlap_Lt_pair; eauto.
+          + eapply no_overlap_mem_perm, Hinj'.
+          + eapply CMatch.
+          + eapply Hangel_bound.
+        - split; eapply mi_inj_mi_perm_perm_Cur_backwards;
+            eauto.
+          + subst; apply Hinj_th.
+          + subst; apply Hinj_lock.
+        - eapply inject_perm_perfect_image_dmap_pair; eauto.
+          + eapply sub_map_implication_dmap_pair; eauto.
+          + eapply full_inject_dmap_pair; eauto.
+            eapply CMatch.
+            eapply join_dmap_valid_pair, Hangel_bound. }
+
+      
+      assert (Hmemval:
+                mi_memval_perm_pair
+                  mu ThreadPerm1
+                  (Mem.mem_contents m1) (Mem.mem_contents m2)).
+      { eapply mi_memval_perm_computeMap_Lt_pair.
+        - split; eapply mi_inj_mi_memval_perm_backwards.
+          + subst; eapply Hinj_th.
+          + subst; eapply Hinj_lock.  
+        - eapply permMapJoin_lt_pair2; eauto. }
+      
+      assert (Hmemval_new:
+                mi_memval_perm_pair mu newThreadPerm1
+                                    (Mem.mem_contents m1) (Mem.mem_contents m2)).
+      { eapply mi_memval_perm_computeMap_Lt_pair.
+        - split; eapply mi_inj_mi_memval_perm_backwards.
+          + subst; eapply Hinj_th.
+          + subst; eapply Hinj_lock.  
+        - eapply permMapJoin_lt_pair2, permMapJoin_pair_comm; eauto. }
+
+      assert (Hmi_perm_inv_perm: (mi_perm_inv_perm_pair
+                                    mu ThreadPerm1
+                                    ThreadPerm2 m1)) by
+          (eapply mi_perm_inv_perm_compute_pair; subst; eauto).
+      
+      assert (Hmi_perm_inv_perm_new: (mi_perm_inv_perm_pair
+                                        mu newThreadPerm1
+                                        newThreadPerm2 m1)).
+      { eapply mi_perm_inv_perm_compute_pair; subst; eauto;
+          eapply inject_empty; eauto. }
+
+      assert (Hinj'': Mem.inject mu
+                                 (restrPermMap Hlt1')
+                                 (restrPermMap Hlt2')).
+      { apply inject_restr; simpl; eauto.
+        - apply Hmi_perm_perm.
+        - apply Hmemval.
+        - apply Hmi_perm_inv_perm. }
+      
+      assert (Hinj1_lk': Mem.inject mu (restrPermMap Hlt1_lk') (restrPermMap Hlt2_lk')).
+      { apply inject_restr; simpl; eauto.
+        - apply Hmi_perm_perm.
+        - apply Hmemval.
+        - apply Hmi_perm_inv_perm. }
+
+      assert (Hinj_new': Mem.inject mu (restrPermMap Hlt1_new) (restrPermMap Hlt2_new)).
+      { apply inject_restr; simpl; eauto.
+        - apply Hmi_perm_perm_new.
+        - apply Hmemval_new.
+        - apply Hmi_perm_inv_perm_new. }
+      
+      assert (Hinj_new_lk': Mem.inject mu (restrPermMap Hlt1_lk_new) (restrPermMap Hlt2_lk_new)).
+      { apply inject_restr; simpl; eauto.
+        - apply Hmi_perm_perm_new.
+        - apply Hmemval_new.
+        - apply Hmi_perm_inv_perm_new. } 
+      
       
       
       (** * 4. Finally we proceed with the goal: existentials. *)
@@ -929,7 +1075,43 @@ Lemma mi_inj_mi_perm_perm_Cur_backwards:
       exists event2, st2'', m2.  
       repeat weak_split. (* 4 goal*)
       - !goal(concur_match _ _ _ _ _ _ ).
-        admit. (* Lemma concur_spawn*)
+        
+        unshelve eapply (concur_match_add_thread hb hb mu _ st1)
+          with (Hlt1:=Hlt1')
+               (Hlt2:=Hlt2')
+               (Hlt1_lk:=Hlt1_lk')
+               (Hlt2_lk:=Hlt2_lk')
+               (Hlt1_new0:=Hlt1_new)
+               (Hlt2_new0:=Hlt2_new)
+               (Hlt1_lk_new0:=Hlt1_lk_new)
+               (Hlt2_lk_new0:=Hlt2_lk_new); eauto;
+          subst ThreadPerm1 ThreadPerm2; simpl.
+        + !goal(perm_surj _ _ _).
+          eapply perm_surj_compute.
+          * eapply CMatch.
+          * eapply inject_perm_perfect_image_dmap; eauto.
+            -- eapply sub_map_implication_dmap; eapply Hangel_bound.
+            -- eapply full_inject_dmap.
+               ++ eapply CMatch.
+               ++ eapply join_dmap_valid; eapply Hangel_bound.
+        + !goal(perm_surj _ _ _).
+          eapply perm_surj_compute.
+          * simpl. 
+            exact (perm_surj_empty _).
+          * eapply inject_perm_perfect_image_dmap; eauto.
+            -- eapply sub_map_implication_dmap; eapply Hangel_bound_new.
+            -- eapply full_inject_dmap.
+               ++ eapply CMatch.
+               ++ eapply join_dmap_valid; eapply Hangel_bound_new.
+        + !goal(invariant _).
+          eapply invariant_add_thread; eauto.
+          reflexivity.
+          apply CMatch.
+        + !context_goal one_thread_match. shelve.
+        + eauto.
+          eapply val_inject_incr.
+          eapply evolution_inject_incr; eauto.
+          eauto.
       - subst event2. repeat econstructor; eauto.
       - !goal (syncStep _ _ _ _ _ _).
         
@@ -937,6 +1119,15 @@ Lemma mi_inj_mi_perm_perm_Cur_backwards:
         (* get the memory and injection *)
 
         subst event2 ; unfold build_release_event.
+
+        (* set the event in the right shape *)
+        match goal with
+          |- syncStep _ _ _ _ _ ?ev =>
+          match type of ev with
+            ?T => evar (ev_new: T);
+                   replace ev with ev_new; unfold ev_new
+          end
+        end.
         
         eapply step_create;
           match goal with
@@ -944,11 +1135,7 @@ Lemma mi_inj_mi_perm_perm_Cur_backwards:
           | |- _ => eauto; try reflexivity
           end.
         + eapply inject_virtue_sub_map_pair'; eauto.
-          * subst; apply Hinj_th.
-          * apply Hangel_bound.
         + eapply inject_virtue_sub_map_pair'; eauto.
-          * subst; apply Hinj_lock.
-          * apply Hangel_bound_new.
         + eapply CMatch.
         + !goal (semantics.at_external _ _ _ = Some (CREATE, _)).
           { simpl. subst ofs2.
@@ -962,41 +1149,92 @@ Lemma mi_inj_mi_perm_perm_Cur_backwards:
             eapply Hjoin_angel2. }
         + { simpl. subst ThreadPerm2 newThreadPerm2 virtue2 virtue_new2.
             eapply Hjoin_angel2. }
+        + subst virtue2 virtue_new2. unfold build_spwan_event.
+          reflexivity.
 
           Unshelve.
-          all: auto.
+          all: eauto.
+          all: try apply empty_LT.
           
-          
-    Admitted.
+          { (*Shelved above*)
+            !context_goal one_thread_match.
+            
 
+            (** *0 . Simplifications to do outside the l emma*)
+
+            set (ThreadPerm1:=computeMap_pair (getThreadR Hcnt1) virtue1).
+
+            
+            (* assert (Hext_rel1': extcall_spawn
+                                  (Genv.globalenv (Ctypes.program_of_program C_program)) 
+                                  (Vptr b1 ofs :: nil) m10
+                                  (Events.Event_acq_rel lev1 (fst virtue1) lev1' :: nil)
+                                  Vundef m1''').
+            { econstructor; try eassumption.
+              econstructor; eauto.
+            } 
+            assert (Hext_rel1: Events.external_call CREATE
+                                                    (Clight.genv_genv Clight_g)
+                                                    (Vptr b1 ofs :: nil)
+                                                    m1 rel_trace Vundef m1''').
+            { simpl; rewrite ReleaseExists.
+              subst rel_trace dpm1; eauto. } *)
+            
+            eapply build_match_compiled; auto.
+            subst st1' st2' st1'' st2''.
+            clean_proofs.
+            
+            eapply CThread_Resume.
+            intros j'' s1' m1''' m2''' lev1' lev2'.
+            intros Hstrict_evolution' (*Hincr'*) Hinterference1' Hinterference2'
+                   Hafter_ext.
+            
+            eapply large_external_diagram; try reflexivity; eauto.
+            - 
+              exact spawn_is_consec.
+            - exact spawn_doesnt_return.
+            - reflexivity.
+            - eapply inject_delta_map_empty.
+            - simpl.
+              
+              rewrite SpawnExists.
+              do 2 (econstructor; eauto).
+              
+            - simpl; rewrite SpawnExists.
+              do 2 (econstructor; eauto).
+            - apply (interference_consecutive_until _ _ _  Hinterference2).
+            - apply (interference_consecutive_until _ _ _ Hinterference2').
+              
+          }
+    Qed.
     
     Lemma spawn_step_diagram:
       let hybrid_sem:= (sem_coresem (HybridSem (Some hb))) in 
       forall virtue1 virtue_new1 (m1 m2 : mem) (tid : nat) cd
-             (mu : meminj) (st1 : ThreadPool (Some hb)) 
-             (st2 : ThreadPool (Some (S hb)))
-             (cnt1 : ThreadPool.containsThread(Sem:=HybridSem _) st1 tid)
-             (cnt2 : containsThread(Sem:=HybridSem _) st2 tid)
-             (c : semC) (b : block) (ofs : int) arg
-             (Hthread_mem1: access_map_equiv (thread_perms _ _ cnt1) (getCurPerm m1))
-             (Hthread_mem2: access_map_equiv (thread_perms _ _ cnt2) (getCurPerm m2))
-             (CMatch: concur_match cd mu st1 m1 st2 m2)
-             (Hvalid_pointer: Mem.perm m1 b (unsigned ofs) Max Nonempty)
-             (Hnot_undef_arg: arg <> Vundef)
-             (Hcode: getThreadC cnt1 = Kblocked c)
-             (Harg : val_inject (Mem.flat_inj (Mem.nextblock m1)) arg arg),
+        (mu : meminj) (st1 : ThreadPool (Some hb)) 
+        (st2 : ThreadPool (Some (S hb)))
+        (cnt1 : ThreadPool.containsThread(Sem:=HybridSem _) st1 tid)
+        (cnt2 : containsThread(Sem:=HybridSem _) st2 tid)
+        (c : semC) (b : block) (ofs : int) arg
+        (Hthread_mem1: access_map_equiv (thread_perms _ _ cnt1) (getCurPerm m1))
+        (Hthread_mem2: access_map_equiv (thread_perms _ _ cnt2) (getCurPerm m2))
+        (CMatch: concur_match cd mu st1 m1 st2 m2)
+        (Hvalid_pointer: Mem.perm m1 b (unsigned ofs) Max Nonempty)
+        (Hnot_undef_arg: arg <> Vundef)
+        (Hcode: getThreadC cnt1 = Kblocked c)
+        (Harg : val_inject (Mem.flat_inj (Mem.nextblock m1)) arg arg),
         let ThreadPerm1:= (computeMap_pair (getThreadR cnt1) virtue1) in
         let newThreadPerm1:= (computeMap_pair (pair0 empty_map) virtue_new1) in
 
         let st1':= (ThreadPool.updThread cnt1 (Kresume c Vundef) ThreadPerm1) in
         let st1'':= (ThreadPool.addThread st1' (Vptr b ofs) arg newThreadPerm1) in
         forall (Hcmpt : mem_compatible  st1'' m1)
-               (Hinv' : invariant st1'')
-               (Hangel_bound: pair21_prop sub_map virtue1 (snd (getMaxPerm m1)))
-               (Hangel_bound_new : pair21_prop sub_map virtue_new1 (snd (getMaxPerm m1)))
-               (Hat_external: semantics.at_external hybrid_sem c m1 =
-                              Some (CREATE, Vptr b ofs :: arg :: nil))
-               (Hjoin_angel: permMapJoin_pair newThreadPerm1 ThreadPerm1 (getThreadR cnt1)),
+          (Hinv' : invariant st1'')
+          (Hangel_bound: pair21_prop sub_map virtue1 (snd (getMaxPerm m1)))
+          (Hangel_bound_new : pair21_prop sub_map virtue_new1 (snd (getMaxPerm m1)))
+          (Hat_external: semantics.at_external hybrid_sem c m1 =
+                         Some (CREATE, Vptr b ofs :: arg :: nil))
+          (Hjoin_angel: permMapJoin_pair newThreadPerm1 ThreadPerm1 (getThreadR cnt1)),
 
         exists evnt2 (st2'' : t) m2',
           let evnt:= build_spwan_event (b, unsigned ofs)
